Makefile
@@ -1,0 +1,31 @@
+COQMAKEFILE := CoqMakefile
+COQMAKE := +$(MAKE) -f $(COQMAKEFILE)
+
+ifeq ($(OS), Windows_NT)
+	UNAME_S := Windows
+else
+	UNAME_S := $(shell uname -s)
+endif
+
+ifeq ($(UNAME_S), Darwin)
+	SED_FLAG := -i ""
+else
+	SED_FLAG := -i
+endif
+
+autosubst2/def.v:
+	autosubst autosubst2/systemf.sig -o autosubst2/def.v -s ucoq
+	mv autosubst2/core.v autosubst2/prop_as_core.v
+	mv autosubst2/unscoped.v autosubst2/prop_as_unscoped.v
+	sed -e "s/Require Import core./Require Import binder.autosubst2.prop_as_core./g" ${SED_FLAG} autosubst2/prop_as_unscoped.v
+	sed -e "s/Require Import core unscoped./Require Import binder.autosubst2.prop_as_core binder.autosubst2.prop_as_unscoped./g" ${SED_FLAG} autosubst2/def.v 
+	sed -e "s/var_ftyp/ftyp_var/g" ${SED_FLAG} autosubst2/def.v 
+	sed -e "s/var_fexp/fexp_var/g" ${SED_FLAG} autosubst2/def.v 
+
+$(COQMAKEFILE):
+	coq_makefile -f _CoqProject -o $(COQMAKEFILE)
+
+coq: $(COQMAKEFILE)
+	+$(MAKE) -f $(COQMAKEFILE) all
+
+.phony: coq autosubst2/def.v
